Simplify termination arguments for captureNext.go

regex/Regex/Backtracker/Basic.lean
@@ -40,6 +40,11 @@ def curr {startIdx : Nat} (bit : BoundedIterator startIdx) (h : bit.hasNext) : C
 
 theorem next_maxIdx {startIdx : Nat} (bit : BoundedIterator startIdx) (h : bit.hasNext) : (bit.next h).maxIdx = bit.maxIdx := rfl
 
+def remainingBytes {startIdx : Nat} (bit : BoundedIterator startIdx) : Nat := bit.it.remainingBytes
+
+theorem next_remainingBytes_lt {startIdx : Nat} (bit : BoundedIterator startIdx) (h : bit.hasNext) : (bit.next h).remainingBytes < bit.remainingBytes := by
+  simp [next, remainingBytes]
+
 end BoundedIterator
 
 structure StackEntry (σ : Strategy) (nfa : NFA) (startIdx maxIdx : Nat) where
@@ -101,24 +106,23 @@ termination_by (nfa.nodes.size * (maxIdx + 1 - startIdx) + 1 - visited.popcount,
 
 def captureNext (σ : Strategy) (nfa : NFA) (wf : nfa.WellFormed) (it : Iterator) : Option σ.Update :=
   let startIdx := it.pos.byteIdx
-  (go startIdx it (Nat.le_refl _) (BitMatrix.zero _ _)).1
-where
-  go (startIdx : Nat) (it : Iterator) (ge : startIdx ≤ it.pos.byteIdx) (visited : BitMatrix nfa.nodes.size (it.toString.endPos.byteIdx + 1 - startIdx)) :
-  Option σ.Update × BitMatrix nfa.nodes.size (it.toString.endPos.byteIdx + 1 - startIdx) :=
   if le : it.pos ≤ it.toString.endPos then
-    let bit : BoundedIterator startIdx := ⟨it, ge, le⟩
-    match captureNextAux σ nfa wf startIdx it.toString.endPos.byteIdx visited [⟨σ.empty, ⟨nfa.start, wf.start_lt⟩, bit, rfl⟩] with
-    | (.some update, visited') => (.some update, visited')
-    | (.none, visited') =>
-      have : it.next.pos.byteIdx ≤ it.toString.endPos.byteIdx + 4 := Nat.le_trans it.next_le_four (by simpa [le])
-      have : it.next.toString.endPos.byteIdx + 4 - it.next.pos.byteIdx < it.toString.endPos.byteIdx + 4 - it.pos.byteIdx := by
-        rw [it.next_toString]
-        have : it.pos.byteIdx < it.next.pos.byteIdx := it.lt_next
-        omega
-      go startIdx it.next (Nat.le_of_lt (Nat.lt_of_le_of_lt ge it.lt_next)) visited'
+    let bit : BoundedIterator startIdx := ⟨it, Nat.le_refl _, le⟩
+    (go startIdx bit (BitMatrix.zero _ _)).1
   else
-    (.none, visited)
-  termination_by it.toString.endPos.byteIdx + 4 - it.pos.byteIdx
+    .none
+where
+  go (startIdx : Nat) (bit : BoundedIterator startIdx) (visited : BitMatrix nfa.nodes.size (bit.maxIdx + 1 - startIdx)) :
+  Option σ.Update × BitMatrix nfa.nodes.size (bit.maxIdx + 1 - startIdx) :=
+  match captureNextAux σ nfa wf startIdx bit.maxIdx visited [⟨σ.empty, ⟨nfa.start, wf.start_lt⟩, bit, rfl⟩] with
+  | (.some update, visited') => (.some update, visited')
+  | (.none, visited') =>
+    if h : bit.hasNext then
+      have : (bit.next h).remainingBytes < bit.remainingBytes := bit.next_remainingBytes_lt h
+      go startIdx (bit.next h) visited'
+    else
+      (.none, visited')
+  termination_by bit.remainingBytes
 
 def captureNextBuf (nfa : NFA) (wf : nfa.WellFormed) (bufferSize : Nat) (it : Iterator) : Option (Buffer bufferSize) :=
   let _ := BufferStrategy bufferSize
